{-# OPTIONS --without-K --exact-split #-}

module extra.final-coalgebras where

open import extra.sequential-limits public

-- Coalgebras for polynomial endofunctors

coalgebra-polynomial-endofunctor-UU :
  (l : Level) {l1 l2 : Level} (A : UU l1) (B : A → UU l2) →
  UU (lsuc l ⊔ l1 ⊔ l2)
coalgebra-polynomial-endofunctor-UU l A B =
  Σ (UU l) (λ X → X → type-polynomial-endofunctor A B X)

type-coalgebra-polynomial-endofunctor :
  {l1 l2 l3 : Level} {A : UU l1} {B : A → UU l2} →
  coalgebra-polynomial-endofunctor-UU l3 A B → UU l3
type-coalgebra-polynomial-endofunctor = pr1

costructure-coalgebra-polynomial-endofunctor :
  {l1 l2 l3 : Level} {A : UU l1} {B : A → UU l2} →
  (X : coalgebra-polynomial-endofunctor-UU l3 A B) →
  type-coalgebra-polynomial-endofunctor X →
  type-polynomial-endofunctor A B (type-coalgebra-polynomial-endofunctor X)
costructure-coalgebra-polynomial-endofunctor = pr2

-- Morphisms of coalgebras for polynomial endofunctors

module _
  {l1 l2 l3 l4 : Level} {A : UU l1} {B : A → UU l2}
  (X : coalgebra-polynomial-endofunctor-UU l3 A B)
  (Y : coalgebra-polynomial-endofunctor-UU l4 A B)
  where
  
  hom-coalgebra-polynomial-endofunctor : UU (l1 ⊔ l2 ⊔ l3 ⊔ l4)
  hom-coalgebra-polynomial-endofunctor =
    Σ ( type-coalgebra-polynomial-endofunctor X →
        type-coalgebra-polynomial-endofunctor Y)
      ( λ h →
        ( ( map-polynomial-endofunctor A B h) ∘
          ( costructure-coalgebra-polynomial-endofunctor X)) ~
        ( costructure-coalgebra-polynomial-endofunctor Y ∘ h))

  map-hom-coalgebra-polynomial-endofunctor :
    (h : hom-coalgebra-polynomial-endofunctor) →
    type-coalgebra-polynomial-endofunctor X →
    type-coalgebra-polynomial-endofunctor Y
  map-hom-coalgebra-polynomial-endofunctor = pr1

  square-hom-coalgebra-polynomial-endofunctor :
    (h : hom-coalgebra-polynomial-endofunctor) →
    ( ( map-polynomial-endofunctor A B
        ( map-hom-coalgebra-polynomial-endofunctor h)) ∘
      ( costructure-coalgebra-polynomial-endofunctor X)) ~
    ( ( costructure-coalgebra-polynomial-endofunctor Y) ∘
      ( map-hom-coalgebra-polynomial-endofunctor h))
  square-hom-coalgebra-polynomial-endofunctor = pr2

  -- We characterize the identity type of hom-coalgebra-polynomial-endofunctor
  
  naturality-htpy-hom-coalgebra-polynomial-endofunctor :
    (f g : hom-coalgebra-polynomial-endofunctor) →
    (H : map-hom-coalgebra-polynomial-endofunctor f ~
         map-hom-coalgebra-polynomial-endofunctor g) →
    UU (l1 ⊔ l2 ⊔ l3 ⊔ l4)
  naturality-htpy-hom-coalgebra-polynomial-endofunctor f g H =
    ( ( ( htpy-polynomial-endofunctor A B H) ·r
        ( costructure-coalgebra-polynomial-endofunctor X)) ∙h
      ( square-hom-coalgebra-polynomial-endofunctor g)) ~
    ( ( square-hom-coalgebra-polynomial-endofunctor f) ∙h
      ( ( costructure-coalgebra-polynomial-endofunctor Y) ·l H))

  htpy-hom-coalgebra-polynomial-endofunctor :
    (f g : hom-coalgebra-polynomial-endofunctor) →
    UU (l1 ⊔ l2 ⊔ l3 ⊔ l4)
  htpy-hom-coalgebra-polynomial-endofunctor f g =
    Σ ( map-hom-coalgebra-polynomial-endofunctor f ~
        map-hom-coalgebra-polynomial-endofunctor g)
      ( naturality-htpy-hom-coalgebra-polynomial-endofunctor f g)

  refl-htpy-hom-coalgebra-polynomial-endofunctor :
    (f : hom-coalgebra-polynomial-endofunctor) →
    htpy-hom-coalgebra-polynomial-endofunctor f f
  refl-htpy-hom-coalgebra-polynomial-endofunctor f =
    pair ( refl-htpy)
         ( ( λ x →
             ap ( concat'
                  ( map-polynomial-endofunctor A B (pr1 f) (pr2 X x))
                  ( pr2 f x))
                ( coh-refl-htpy-polynomial-endofunctor A B
                  ( pr1 f)
                  ( costructure-coalgebra-polynomial-endofunctor X x))) ∙h
           ( inv-htpy right-unit-htpy))

  htpy-hom-coalgebra-polynomial-endofunctor-eq :
    (f g : hom-coalgebra-polynomial-endofunctor) →
    Id f g → htpy-hom-coalgebra-polynomial-endofunctor f g
  htpy-hom-coalgebra-polynomial-endofunctor-eq f .f refl =
    refl-htpy-hom-coalgebra-polynomial-endofunctor f

  is-contr-total-htpy-hom-coalgebra-polynomial-endofunctor :
    (f : hom-coalgebra-polynomial-endofunctor) →
    is-contr
      ( Σ ( hom-coalgebra-polynomial-endofunctor)
          ( htpy-hom-coalgebra-polynomial-endofunctor f))
  is-contr-total-htpy-hom-coalgebra-polynomial-endofunctor f =
    is-contr-total-Eq-structure
      ( λ g G →
        naturality-htpy-hom-coalgebra-polynomial-endofunctor f (pair g G))
      ( is-contr-total-htpy (map-hom-coalgebra-polynomial-endofunctor f))
      ( pair (map-hom-coalgebra-polynomial-endofunctor f) refl-htpy)
      ( is-contr-equiv
        ( Σ ( ( ( map-polynomial-endofunctor A B
                  ( map-hom-coalgebra-polynomial-endofunctor f)) ∘
                ( costructure-coalgebra-polynomial-endofunctor X)) ~
              ( ( costructure-coalgebra-polynomial-endofunctor Y) ∘
                ( map-hom-coalgebra-polynomial-endofunctor f)))
            ( λ H → H ~ (square-hom-coalgebra-polynomial-endofunctor f)))
        ( equiv-tot
          ( λ H →
            ( equiv-concat-htpy
              ( inv-htpy
                ( λ x →
                  ap ( concat'
                       ( map-polynomial-endofunctor A B (pr1 f) (pr2 X x))
                       ( H x))
                     ( coh-refl-htpy-polynomial-endofunctor A B
                       ( pr1 f)
                       ( costructure-coalgebra-polynomial-endofunctor X x))))
              ( square-hom-coalgebra-polynomial-endofunctor f)) ∘e
            ( equiv-concat-htpy'
              ( ( ( htpy-polynomial-endofunctor A B
                    ( refl-htpy
                      { f = map-hom-coalgebra-polynomial-endofunctor f})) ·r
                  ( costructure-coalgebra-polynomial-endofunctor X)) ∙h
                ( H))
              ( right-unit-htpy))))
        ( is-contr-total-htpy'
          ( square-hom-coalgebra-polynomial-endofunctor f)))

is-equiv-htpy-hom-coalgebra-polynomial-endofunctor-eq :
  {l1 l2 l3 l4 : Level} {A : UU l1} {B : A → UU l2} →
  (X : coalgebra-polynomial-endofunctor-UU l3 A B) →
  (Y : coalgebra-polynomial-endofunctor-UU l4 A B) →
  (f g : hom-coalgebra-polynomial-endofunctor X Y) →
  is-equiv (htpy-hom-coalgebra-polynomial-endofunctor-eq X Y f g)
is-equiv-htpy-hom-coalgebra-polynomial-endofunctor-eq X Y f =
  fundamental-theorem-id f
    ( refl-htpy-hom-coalgebra-polynomial-endofunctor X Y f)
    ( is-contr-total-htpy-hom-coalgebra-polynomial-endofunctor X Y f)
    ( htpy-hom-coalgebra-polynomial-endofunctor-eq X Y f)

--------------------------------------------------------------------------------

{- We define the underlying type of the final coalgebra of a polynomial 
   endofunctor -}

type-coseq-final-coalgebra-polynomial-endofunctor :
  {l1 l2 : Level} (A : UU l1) (B : A → UU l2) → ℕ → UU (l1 ⊔ l2)
type-coseq-final-coalgebra-polynomial-endofunctor A B zero-ℕ =
  raise _ unit
type-coseq-final-coalgebra-polynomial-endofunctor A B (succ-ℕ n) =
  type-polynomial-endofunctor A B
    ( type-coseq-final-coalgebra-polynomial-endofunctor A B n)

map-coseq-final-coalgebra-polynomial-endofunctor :
  {l1 l2 : Level} (A : UU l1) (B : A → UU l2) (n : ℕ) →
  type-coseq-final-coalgebra-polynomial-endofunctor A B (succ-ℕ n) →
  type-coseq-final-coalgebra-polynomial-endofunctor A B n
map-coseq-final-coalgebra-polynomial-endofunctor A B zero-ℕ x =
  raise-star
map-coseq-final-coalgebra-polynomial-endofunctor A B (succ-ℕ n) =
  map-polynomial-endofunctor A B
    ( map-coseq-final-coalgebra-polynomial-endofunctor A B n)

coseq-final-coalgebra-polynomial-endofunctor :
  {l1 l2 : Level} (A : UU l1) (B : A → UU l2) → Coseq-UU (l1 ⊔ l2)
coseq-final-coalgebra-polynomial-endofunctor A B =
  pair ( type-coseq-final-coalgebra-polynomial-endofunctor A B)
       ( map-coseq-final-coalgebra-polynomial-endofunctor A B)

type-final-coalgebra-polynomial-endofunctor :
  {l1 l2 : Level} (A : UU l1) (B : A → UU l2) → UU (l1 ⊔ l2)
type-final-coalgebra-polynomial-endofunctor A B =
  limit-Coseq
    ( coseq-final-coalgebra-polynomial-endofunctor A B)

{-
point-type-final-coalgebra-polynomial-endofunctor :
  {l1 l2 : Level} {A : UU l1} {B : A → UU l2} →
  (x : type-final-coalgebra-polynomial-endofunctor A B) (n : ℕ) →
  type-coseq-final-coalgebra-polynomial-endofunctor A B n
point-type-final-coalgebra-polynomial-endofunctor {A = A} {B} =
  limit-Coseq
    ( coseq-final-coalgebra-polynomial-endofunctor A B)

path-type-final-coalgebra-polynomial-endofunctor :
  {l1 l2 : Level} {A : UU l1} {B : A → UU l2} →
  (x : type-final-coalgebra-polynomial-endofunctor A B) (n : ℕ) →
  Id ( map-coseq-final-coalgebra-polynomial-endofunctor A B n
       ( point-type-final-coalgebra-polynomial-endofunctor x (succ-ℕ n)))
     ( point-type-final-coalgebra-polynomial-endofunctor x n)
path-type-final-coalgebra-polynomial-endofunctor {A = A} {B} =
  path-limit-Coseq
    ( coseq-final-coalgebra-polynomial-endofunctor A B)

cone-final-coalgebra-polynomial-endofunctor :
  {l1 l2 : Level} (A : UU l1) (B : A → UU l2) →
  cone-Coseq (coseq-final-coalgebra-polynomial-endofunctor A B)
             (type-final-coalgebra-polynomial-endofunctor A B)
cone-final-coalgebra-polynomial-endofunctor A B =
  cone-limit-Coseq
    ( coseq-final-coalgebra-polynomial-endofunctor A B)

universal-property-cone-final-coalgebra-polynomial-endofunctor :
  ( l : Level) {l1 l2 : Level} (A : UU l1) (B : A → UU l2) → 
  universal-property-limit-Coseq l
    ( coseq-final-coalgebra-polynomial-endofunctor A B)
    ( cone-final-coalgebra-polynomial-endofunctor A B)
universal-property-cone-final-coalgebra-polynomial-endofunctor l A B =
  universal-property-limit-limit-Coseq l
    ( coseq-final-coalgebra-polynomial-endofunctor A B)

--------------------------------------------------------------------------------

{- We define the costructure on the final coalgebra -}

costructure-final-coalgebra-polynomial-endofunctor :
  {l1 l2 : Level} (A : UU l1) (B : A → UU l2) →
  type-final-coalgebra-polynomial-endofunctor A B →
  type-polynomial-endofunctor A B
    ( type-final-coalgebra-polynomial-endofunctor A B)
costructure-final-coalgebra-polynomial-endofunctor A B =
  map-inv-equiv
    ( ( equiv-limit-shift-Coseq
        ( coseq-final-coalgebra-polynomial-endofunctor A B)) ∘e
      {!!})  

head-type-final-coalgebra-polynomial-endofunctor :
  {l1 l2 : Level} {A : UU l1} {B : A → UU l2} →
  type-final-coalgebra-polynomial-endofunctor A B → A
head-type-final-coalgebra-polynomial-endofunctor x = pr1 (pr1 x one-ℕ)

eq-head-type-final-coalgebra-polynomial-endofunctor :
  {l1 l2 : Level} {A : UU l1} {B : A → UU l2} →
  (x : type-final-coalgebra-polynomial-endofunctor A B) (n : ℕ) →
  Id ( pr1 (point-type-final-coalgebra-polynomial-endofunctor x (succ-ℕ n)))
     ( head-type-final-coalgebra-polynomial-endofunctor x)
eq-head-type-final-coalgebra-polynomial-endofunctor x zero-ℕ = refl
eq-head-type-final-coalgebra-polynomial-endofunctor x (succ-ℕ n) =
  ( ap pr1 (path-type-final-coalgebra-polynomial-endofunctor x (succ-ℕ n))) ∙
  ( eq-head-type-final-coalgebra-polynomial-endofunctor x n)

points-tail-type-final-coalgebra-polynomial-endofunctor :
  {l1 l2 : Level} {A : UU l1} {B : A → UU l2} →
  (x : type-final-coalgebra-polynomial-endofunctor A B) →
  B (head-type-final-coalgebra-polynomial-endofunctor x) →
  (n : ℕ) → type-coseq-final-coalgebra-polynomial-endofunctor A B n
points-tail-type-final-coalgebra-polynomial-endofunctor {A = A} {B} x y n =
  pr2 ( point-type-final-coalgebra-polynomial-endofunctor x (succ-ℕ n))
      ( inv-tr B (eq-head-type-final-coalgebra-polynomial-endofunctor x n) y)

tail-type-final-coalgebra-polynomial-endofunctor :
  {l1 l2 : Level} {A : UU l1} {B : A → UU l2} →
  (x : type-final-coalgebra-polynomial-endofunctor A B) →
  B (head-type-final-coalgebra-polynomial-endofunctor x) →
  type-final-coalgebra-polynomial-endofunctor A B
tail-type-final-coalgebra-polynomial-endofunctor x y =
  pair
    ( points-tail-type-final-coalgebra-polynomial-endofunctor x y)
    {!!}
-}
