{-# OPTIONS --without-K --exact-split #-}

module book.14-propositional-truncation where

import book.13-function-extensionality-solutions
open book.13-function-extensionality-solutions public

--------------------------------------------------------------------------------

-- Section 14 Propositional truncations and the image of a map

--------------------------------------------------------------------------------

-- Section 14.1 Propositional truncations

-- Definition 14.1.1

precomp-Prop :
  { l1 l2 l3 : Level} {A : UU l1} (P : UU-Prop l2) →
  (A → type-Prop P) → (Q : UU-Prop l3) →
  (type-hom-Prop P Q) → (A → type-Prop Q)
precomp-Prop P f Q g = g ∘ f

is-propositional-truncation :
  ( l : Level) {l1 l2 : Level} {A : UU l1} (P : UU-Prop l2) →
  ( A → type-Prop P) → UU (lsuc l ⊔ l1 ⊔ l2)
is-propositional-truncation l P f =
  (Q : UU-Prop l) → is-equiv (precomp-Prop P f Q)

-- Remark 14.2

universal-property-propositional-truncation :
  ( l : Level) {l1 l2 : Level} {A : UU l1}
  (P : UU-Prop l2) (f : A → type-Prop P) → UU (lsuc l ⊔ l1 ⊔ l2)
universal-property-propositional-truncation l {A = A} P f =
  (Q : UU-Prop l) (g : A → type-Prop Q) →
  is-contr (Σ (type-hom-Prop P Q) (λ h → (h ∘ f) ~  g))

universal-property-is-propositional-truncation :
  (l : Level) {l1 l2 : Level} {A : UU l1}
  (P : UU-Prop l2) (f : A → type-Prop P) →
  is-propositional-truncation l P f →
  universal-property-propositional-truncation l P f
universal-property-is-propositional-truncation l P f is-ptr-f Q g =
  is-contr-equiv'
    ( Σ (type-hom-Prop P Q) (λ h → Id (h ∘ f) g))
    ( equiv-tot (λ h → equiv-funext))
    ( is-contr-map-is-equiv (is-ptr-f Q) g)

map-is-propositional-truncation :
  {l1 l2 l3 : Level} {A : UU l1} (P : UU-Prop l2) (f : A → type-Prop P) →
  ({l : Level} → is-propositional-truncation l P f) →
  (Q : UU-Prop l3) (g : A → type-Prop Q) → type-hom-Prop P Q
map-is-propositional-truncation P f is-ptr-f Q g =
  pr1
    ( center
      ( universal-property-is-propositional-truncation _ P f is-ptr-f Q g))

htpy-is-propositional-truncation :
  {l1 l2 l3 : Level} {A : UU l1} (P : UU-Prop l2) (f : A → type-Prop P) →
  (is-ptr-f : {l : Level} → is-propositional-truncation l P f) →
  (Q : UU-Prop l3) (g : A → type-Prop Q) →
  ((map-is-propositional-truncation P f is-ptr-f Q g) ∘ f) ~ g
htpy-is-propositional-truncation P f is-ptr-f Q g =
  pr2
    ( center
      ( universal-property-is-propositional-truncation _ P f is-ptr-f Q g))

is-propositional-truncation-universal-property :
  (l : Level) {l1 l2 : Level} {A : UU l1}
  (P : UU-Prop l2) (f : A → type-Prop P) →
  universal-property-propositional-truncation l P f →
  is-propositional-truncation l P f
is-propositional-truncation-universal-property l P f up-f Q =
  is-equiv-is-contr-map
    ( λ g → is-contr-equiv
      ( Σ (type-hom-Prop P Q) (λ h → (h ∘ f) ~ g))
      ( equiv-tot (λ h → equiv-funext))
      ( up-f Q g))

-- Remark 14.1.3

extension-property-propositional-truncation :
  ( l : Level) {l1 l2 : Level} {A : UU l1} (P : UU-Prop l2) →
  ( A → type-Prop P) → UU (lsuc l ⊔ l1 ⊔ l2)
extension-property-propositional-truncation l {A = A} P f =
  (Q : UU-Prop l) → (A → type-Prop Q) → (type-hom-Prop P Q)

is-propositional-truncation-extension-property :
  { l1 l2 : Level} {A : UU l1} (P : UU-Prop l2)
  ( f : A → type-Prop P) →
  ( {l : Level} → extension-property-propositional-truncation l P f) →
  ( {l : Level} → is-propositional-truncation l P f)
is-propositional-truncation-extension-property P f up-P {l} Q =
  is-equiv-is-prop
    ( is-prop-Π (λ x → is-prop-type-Prop Q))
    ( is-prop-Π (λ x → is-prop-type-Prop Q))
    ( up-P Q)

-- Proposition 14.1.4

abstract
  is-equiv-is-equiv-precomp-Prop :
    {l1 l2 : Level} (P : UU-Prop l1) (Q : UU-Prop l2) (f : type-hom-Prop P Q) →
    ({l : Level} → is-propositional-truncation l Q f) → is-equiv f
  is-equiv-is-equiv-precomp-Prop P Q f H =
    is-equiv-is-prop
      ( is-prop-type-Prop P)
      ( is-prop-type-Prop Q)
      ( map-inv-is-equiv (H P) id)

is-equiv-is-ptruncation-is-ptruncation :
  {l1 l2 l3 : Level} {A : UU l1} (P : UU-Prop l2) (P' : UU-Prop l3)
  (f : A → type-Prop P) (f' : A → type-Prop P')
  (h : type-hom-Prop P P') (H : (h ∘ f) ~ f') →
  ({l : Level} → is-propositional-truncation l P f) →
  ({l : Level} → is-propositional-truncation l P' f') →
  is-equiv h
is-equiv-is-ptruncation-is-ptruncation P P' f f' h H is-ptr-P is-ptr-P' =
  is-equiv-is-prop
    ( is-prop-type-Prop P)
    ( is-prop-type-Prop P')
    ( map-inv-is-equiv (is-ptr-P' P) f)

is-ptruncation-is-ptruncation-is-equiv :
  {l1 l2 l3 : Level} {A : UU l1} (P : UU-Prop l2) (P' : UU-Prop l3)
  (f : A → type-Prop P) (f' : A → type-Prop P') (h : type-hom-Prop P P') →
  is-equiv h → ({l : Level} → is-propositional-truncation l P f) →
  ({l : Level} → is-propositional-truncation l P' f')
is-ptruncation-is-ptruncation-is-equiv P P' f f' h is-equiv-h is-ptr-f =
  is-propositional-truncation-extension-property P' f'
    ( λ R g →
      ( map-is-propositional-truncation P f is-ptr-f R g) ∘
      ( map-inv-is-equiv is-equiv-h))

is-ptruncation-is-equiv-is-ptruncation :
  {l1 l2 l3 : Level} {A : UU l1} (P : UU-Prop l2) (P' : UU-Prop l3)
  (f : A → type-Prop P) (f' : A → type-Prop P') (h : type-hom-Prop P P') →
  ({l : Level} → is-propositional-truncation l P' f') → is-equiv h →
  ({l : Level} → is-propositional-truncation l P f)
is-ptruncation-is-equiv-is-ptruncation P P' f f' h is-ptr-f' is-equiv-h =
  is-propositional-truncation-extension-property P f
    ( λ R g → (map-is-propositional-truncation P' f' is-ptr-f' R g) ∘ h)

is-uniquely-unique-propositional-truncation :
  {l1 l2 l3 : Level} {A : UU l1} (P : UU-Prop l2) (P' : UU-Prop l3)
  (f : A → type-Prop P) (f' : A → type-Prop P') →
  ({l : Level} → is-propositional-truncation l P f) →
  ({l : Level} → is-propositional-truncation l P' f') →
  is-contr (Σ (type-equiv-Prop P P') (λ e → (map-equiv e ∘ f) ~ f'))
is-uniquely-unique-propositional-truncation P P' f f' is-ptr-f is-ptr-f' =
  is-contr-total-Eq-substructure
    ( universal-property-is-propositional-truncation _ P f is-ptr-f P' f')
    ( is-subtype-is-equiv)
    ( map-is-propositional-truncation P f is-ptr-f P' f')
    ( htpy-is-propositional-truncation P f is-ptr-f P' f')
    ( is-equiv-is-ptruncation-is-ptruncation  P P' f f'
      ( map-is-propositional-truncation P f is-ptr-f P' f')
      ( htpy-is-propositional-truncation P f is-ptr-f P' f')
      ( λ {l} → is-ptr-f)
      ( λ {l} → is-ptr-f'))

--------------------------------------------------------------------------------

-- Section 14.2 Propositional truncations as higher inductive types

-- Axiom 14.1.8

-- The formation rule

postulate type-trunc-Prop : {l : Level} → UU l → UU l

-- The constructors

postulate unit-trunc-Prop : {l : Level} {A : UU l} → A → type-trunc-Prop A

postulate
  all-elements-equal-type-trunc-Prop :
    {l : Level} {A : UU l} → all-elements-equal (type-trunc-Prop A)

-- Lemma 14.2.1

is-prop-type-trunc-Prop : {l : Level} {A : UU l} → is-prop (type-trunc-Prop A)
is-prop-type-trunc-Prop {l} {A} =
  is-prop-all-elements-equal all-elements-equal-type-trunc-Prop

trunc-Prop : {l : Level} → UU l → UU-Prop l
trunc-Prop A = pair (type-trunc-Prop A) is-prop-type-trunc-Prop

-- The induction principle

-- Definition 14.2.2

postulate
  ind-trunc-Prop' :
    {l l1 : Level} {A : UU l1} (P : type-trunc-Prop A → UU l)
    (f : (x : A) → P (unit-trunc-Prop x))
    (g : (x y : type-trunc-Prop A) (u : P x) (v : P y) →
         Id (tr P (all-elements-equal-type-trunc-Prop x y) u) v) →
    (x : type-trunc-Prop A) → P x

is-prop-condition-ind-trunc-Prop' :
  {l1 l2 : Level} {A : UU l1} {P : type-trunc-Prop A → UU l2} →
  ( (x y : type-trunc-Prop A) (u : P x) (v : P y) →
    Id (tr P (all-elements-equal-type-trunc-Prop x y) u) v) →
  (x : type-trunc-Prop A) → is-prop (P x)
is-prop-condition-ind-trunc-Prop' {P = P} H x =
  is-prop-all-elements-equal
    ( λ u v →
      ( ap ( λ γ → tr P γ u)
           ( eq-is-contr (is-prop-type-trunc-Prop x x))) ∙
      ( H x x u v))

ind-trunc-Prop :
  {l l1 : Level} {A : UU l1} (P : type-trunc-Prop A → UU-Prop l) →
  ((x : A) → type-Prop (P (unit-trunc-Prop x))) →
  (( y : type-trunc-Prop A) → type-Prop (P y))
ind-trunc-Prop P f =
  ind-trunc-Prop' (type-Prop ∘ P) f
    ( λ x y u v → eq-is-prop (is-prop-type-Prop (P y))) 

-- The computation rules

comp-trunc-Prop :
  {l l1 : Level} {A : UU l1} (P : type-trunc-Prop A → UU-Prop l) →
  ((precomp-Π unit-trunc-Prop (type-Prop ∘ P)) ∘ ind-trunc-Prop P) ~ id
comp-trunc-Prop P h =
  eq-is-prop (is-prop-Π (λ x → is-prop-type-Prop (P (unit-trunc-Prop x))))

--------------------------------------------------------------------------------

-- Theorem 14.2.3

is-propositional-truncation-trunc-Prop :
  {l1 l2 : Level} (A : UU l1) →
  is-propositional-truncation l2 (trunc-Prop A) unit-trunc-Prop
is-propositional-truncation-trunc-Prop A =
  is-propositional-truncation-extension-property
    ( trunc-Prop A)
    ( unit-trunc-Prop)
    ( λ {l} Q → ind-trunc-Prop (λ x → Q))

universal-property-trunc-Prop : {l1 l2 : Level} (A : UU l1) →
  universal-property-propositional-truncation l2
    ( trunc-Prop A)
    ( unit-trunc-Prop)
universal-property-trunc-Prop A =
  universal-property-is-propositional-truncation _
    ( trunc-Prop A)
    ( unit-trunc-Prop)
    ( is-propositional-truncation-trunc-Prop A)

map-universal-property-trunc-Prop :
  {l1 l2 : Level} {A : UU l1} (P : UU-Prop l2) →
  (A → type-Prop P) → type-hom-Prop (trunc-Prop A) P
map-universal-property-trunc-Prop {A = A} P f =
  map-is-propositional-truncation
    ( trunc-Prop A)
    ( unit-trunc-Prop)
    ( is-propositional-truncation-trunc-Prop A)
    ( P)
    ( f)

apply-universal-property-trunc-Prop :
  {l1 l2 : Level} {A : UU l1} (t : type-trunc-Prop A) (P : UU-Prop l2) →
  (A → type-Prop P) → type-Prop P
apply-universal-property-trunc-Prop t P f =
  map-universal-property-trunc-Prop P f t

-- Proposition 14.2.4

unique-functor-trunc-Prop :
  {l1 l2 : Level} {A : UU l1} {B : UU l2} (f : A → B) →
  is-contr
    ( Σ ( type-hom-Prop (trunc-Prop A) (trunc-Prop B))
        ( λ h → (h ∘ unit-trunc-Prop) ~ (unit-trunc-Prop ∘ f)))
unique-functor-trunc-Prop {l1} {l2} {A} {B} f =
  universal-property-trunc-Prop A (trunc-Prop B) (unit-trunc-Prop ∘ f)

functor-trunc-Prop :
  {l1 l2 : Level} {A : UU l1} {B : UU l2} →
  (A → B) → type-hom-Prop (trunc-Prop A) (trunc-Prop B)
functor-trunc-Prop f =
  pr1 (center (unique-functor-trunc-Prop f))

htpy-functor-trunc-Prop :
  { l1 l2 : Level} {A : UU l1} {B : UU l2} (f : A → B) →
  ( (functor-trunc-Prop f) ∘ unit-trunc-Prop) ~ (unit-trunc-Prop ∘ f)
htpy-functor-trunc-Prop f =
  pr2 (center (unique-functor-trunc-Prop f))

htpy-uniqueness-functor-trunc-Prop :
  { l1 l2 : Level} {A : UU l1} {B : UU l2} (f : A → B) →
  ( h : type-hom-Prop (trunc-Prop A) (trunc-Prop B)) →
  ( ( h ∘ unit-trunc-Prop) ~ (unit-trunc-Prop ∘ f)) →
  (functor-trunc-Prop f) ~ h
htpy-uniqueness-functor-trunc-Prop f h H =
  htpy-eq (ap pr1 (contraction (unique-functor-trunc-Prop f) (pair h H)))

id-functor-trunc-Prop :
  { l1 : Level} {A : UU l1} → functor-trunc-Prop (id {A = A}) ~ id
id-functor-trunc-Prop {l1} {A} =
  htpy-uniqueness-functor-trunc-Prop id id refl-htpy

comp-functor-trunc-Prop :
  { l1 l2 l3 : Level} {A : UU l1} {B : UU l2} {C : UU l3}
  ( g : B → C) (f : A → B) →
  ( functor-trunc-Prop (g ∘ f)) ~
  ( (functor-trunc-Prop g) ∘ (functor-trunc-Prop f))
comp-functor-trunc-Prop g f =
  htpy-uniqueness-functor-trunc-Prop
    ( g ∘ f)
    ( (functor-trunc-Prop g) ∘ (functor-trunc-Prop f))
    ( ( (functor-trunc-Prop g) ·l (htpy-functor-trunc-Prop f)) ∙h
      ( ( htpy-functor-trunc-Prop g) ·r f))

map-equiv-trunc-Prop :
  {l1 l2 : Level} {A : UU l1} {B : UU l2} →
  (A ≃ B) → type-trunc-Prop A → type-trunc-Prop B
map-equiv-trunc-Prop e = functor-trunc-Prop (map-equiv e)

map-inv-equiv-trunc-Prop :
  {l1 l2 : Level} {A : UU l1} {B : UU l2} →
  (A ≃ B) → type-trunc-Prop B → type-trunc-Prop A
map-inv-equiv-trunc-Prop e = map-equiv-trunc-Prop (inv-equiv e)

equiv-trunc-Prop :
  {l1 l2 : Level} {A : UU l1} {B : UU l2} →
  (A ≃ B) → (type-trunc-Prop A ≃ type-trunc-Prop B)
equiv-trunc-Prop e =
  pair
    ( map-equiv-trunc-Prop e)
    ( is-equiv-is-prop
      ( is-prop-type-trunc-Prop)
      ( is-prop-type-trunc-Prop)
      ( map-inv-equiv-trunc-Prop e))

--------------------------------------------------------------------------------

-- Section 14.3 Propositional truncations as higher inductive types

-- Definition 14.3.1

case-paths-induction-principle-propositional-truncation :
  { l : Level} {l1 l2 : Level} {A : UU l1}
  ( P : UU-Prop l2) (α : (p q : type-Prop P) → Id p q) (f : A → type-Prop P) →
  ( B : type-Prop P → UU l) → UU (l ⊔ l2)
case-paths-induction-principle-propositional-truncation P α f B =
  (p q : type-Prop P) (x : B p) (y : B q) → Id (tr B (α p q) x) y
  
induction-principle-propositional-truncation :
  (l : Level) {l1 l2 : Level} {A : UU l1}
  (P : UU-Prop l2) (α : (p q : type-Prop P) → Id p q) (f : A → type-Prop P) →
  UU (lsuc l ⊔ l1 ⊔ l2)
induction-principle-propositional-truncation l {l1} {l2} {A} P α f =
  ( B : type-Prop P → UU l) →
  ( g : (x : A) → (B (f x))) →
  ( β : case-paths-induction-principle-propositional-truncation P α f B) →
  Σ ((p : type-Prop P) → B p) (λ h → (x : A) → Id (h (f x)) (g x))

-- Lemma 14.3.2

is-prop-case-paths-induction-principle-propositional-truncation :
  { l : Level} {l1 l2 : Level} {A : UU l1}
  ( P : UU-Prop l2) (α : (p q : type-Prop P) → Id p q) (f : A → type-Prop P) →
  ( B : type-Prop P → UU l) →
  case-paths-induction-principle-propositional-truncation P α f B →
  ( p : type-Prop P) → is-prop (B p)
is-prop-case-paths-induction-principle-propositional-truncation P α f B β p =
  is-prop-is-proof-irrelevant (λ x → pair (tr B (α p p) x) (β p p x))

case-paths-induction-principle-propositional-truncation-is-prop :
  { l : Level} {l1 l2 : Level} {A : UU l1}
  ( P : UU-Prop l2) (α : (p q : type-Prop P) → Id p q) (f : A → type-Prop P) →
  ( B : type-Prop P → UU l) →
  ( (p : type-Prop P) → is-prop (B p)) →
  case-paths-induction-principle-propositional-truncation P α f B
case-paths-induction-principle-propositional-truncation-is-prop
  P α f B is-prop-B p q x y =
  eq-is-prop (is-prop-B q)

--------------------------------------------------------------------------------

-- Section 14.3 Logic in type theory

-- Conjunction

conj-Prop = prod-Prop

type-conj-Prop :
  {l1 l2 : Level} → UU-Prop l1 → UU-Prop l2 → UU (l1 ⊔ l2)
type-conj-Prop P Q = type-Prop (conj-Prop P Q)

is-prop-type-conj-Prop :
  {l1 l2 : Level} (P : UU-Prop l1) (Q : UU-Prop l2) →
  is-prop (type-conj-Prop P Q)
is-prop-type-conj-Prop P Q = is-prop-type-Prop (conj-Prop P Q)

intro-conj-Prop :
  {l1 l2 : Level} (P : UU-Prop l1) (Q : UU-Prop l2) →
  type-Prop P → type-Prop Q → type-conj-Prop P Q
intro-conj-Prop P Q = pair

-- Disjunction

disj-Prop :
  {l1 l2 : Level} → UU-Prop l1 → UU-Prop l2 → UU-Prop (l1 ⊔ l2)
disj-Prop P Q = trunc-Prop (coprod (type-Prop P) (type-Prop Q))

type-disj-Prop :
  {l1 l2 : Level} → UU-Prop l1 → UU-Prop l2 → UU (l1 ⊔ l2)
type-disj-Prop P Q = type-Prop (disj-Prop P Q)

is-prop-type-disj-Prop :
  {l1 l2 : Level} (P : UU-Prop l1) (Q : UU-Prop l2) →
  is-prop (type-disj-Prop P Q)
is-prop-type-disj-Prop P Q = is-prop-type-Prop (disj-Prop P Q)

inl-disj-Prop :
  {l1 l2 : Level} (P : UU-Prop l1) (Q : UU-Prop l2) →
  type-hom-Prop P (disj-Prop P Q)
inl-disj-Prop P Q = unit-trunc-Prop ∘ inl

inr-disj-Prop :
  {l1 l2 : Level} (P : UU-Prop l1) (Q : UU-Prop l2) →
  type-hom-Prop Q (disj-Prop P Q)
inr-disj-Prop P Q = unit-trunc-Prop ∘ inr

-- Theorem

ev-disj-Prop :
  {l1 l2 l3 : Level} (P : UU-Prop l1) (Q : UU-Prop l2) (R : UU-Prop l3) →
  type-hom-Prop
    ( hom-Prop (disj-Prop P Q) R)
    ( conj-Prop (hom-Prop P R) (hom-Prop Q R))
ev-disj-Prop P Q R h =
  pair (h ∘ (inl-disj-Prop P Q)) (h ∘ (inr-disj-Prop P Q))

inv-ev-disj-Prop :
  {l1 l2 l3 : Level} (P : UU-Prop l1) (Q : UU-Prop l2) (R : UU-Prop l3) →
  type-hom-Prop
    ( conj-Prop (hom-Prop P R) (hom-Prop Q R))
    ( hom-Prop (disj-Prop P Q) R)
inv-ev-disj-Prop P Q R (pair f g) =
  map-universal-property-trunc-Prop R (ind-coprod (λ t → type-Prop R) f g)

is-equiv-ev-disj-Prop :
  {l1 l2 l3 : Level} (P : UU-Prop l1) (Q : UU-Prop l2) (R : UU-Prop l3) →
  is-equiv (ev-disj-Prop P Q R)
is-equiv-ev-disj-Prop P Q R =
  is-equiv-is-prop
    ( is-prop-type-Prop (hom-Prop (disj-Prop P Q) R))
    ( is-prop-type-Prop (conj-Prop (hom-Prop P R) (hom-Prop Q R)))
    ( inv-ev-disj-Prop P Q R)

-- Existential quantification

exists-Prop :
  {l1 l2 : Level} {A : UU l1} (P : A → UU-Prop l2) → UU-Prop (l1 ⊔ l2)
exists-Prop {l1} {l2} {A} P = trunc-Prop (Σ A (λ x → type-Prop (P x)))

exists :
  {l1 l2 : Level} {A : UU l1} (P : A → UU-Prop l2) → UU (l1 ⊔ l2)
exists P = type-Prop (exists-Prop P)

is-prop-exists :
  {l1 l2 : Level} {A : UU l1} (P : A → UU-Prop l2) → is-prop (exists P)
is-prop-exists P = is-prop-type-Prop (exists-Prop P)

intro-exists :
  {l1 l2 : Level} {A : UU l1} (P : A → UU-Prop l2) →
  (x : A) → type-Prop (P x) → exists P
intro-exists {A = A} P x p = unit-trunc-Prop (pair x p)

∃-Prop :
  {l1 l2 : Level} {A : UU l1} (B : A → UU l2) → UU-Prop (l1 ⊔ l2)
∃-Prop {A = A} B = trunc-Prop (Σ A B)

∃ :
  {l1 l2 : Level} {A : UU l1} (B : A → UU l2) → UU (l1 ⊔ l2)
∃ B = type-Prop (∃-Prop B)

is-prop-∃ :
  {l1 l2 : Level} {A : UU l1} (B : A → UU l2) → is-prop (∃ B)
is-prop-∃ B = is-prop-type-Prop (∃-Prop B)

intro-∃ :
  {l1 l2 : Level} {A : UU l1} {B : A → UU l2} (a : A) (b : B a) →
  ∃ B
intro-∃ a b = unit-trunc-Prop (pair a b)

-- Proposition

ev-intro-exists-Prop :
  {l1 l2 l3 : Level} {A : UU l1} (P : A → UU-Prop l2) (Q : UU-Prop l3) →
  type-hom-Prop (exists-Prop P) Q → (x : A) → type-hom-Prop (P x) Q
ev-intro-exists-Prop P Q H x p = H (intro-exists P x p)

elim-exists-Prop :
  {l1 l2 l3 : Level} {A : UU l1} (P : A → UU-Prop l2) (Q : UU-Prop l3) →
  ((x : A) → type-hom-Prop (P x) Q) → type-hom-Prop (exists-Prop P) Q
elim-exists-Prop {A = A} P Q f =
  map-universal-property-trunc-Prop Q (ind-Σ f)

is-equiv-ev-intro-exists-Prop :
  {l1 l2 l3 : Level} {A : UU l1} (P : A → UU-Prop l2) (Q : UU-Prop l3) →
  is-equiv (ev-intro-exists-Prop P Q)
is-equiv-ev-intro-exists-Prop P Q =
  is-equiv-is-prop
    ( is-prop-type-hom-Prop (exists-Prop P) Q)
    ( is-prop-Π ((λ x → is-prop-type-hom-Prop (P x) Q)))
    ( elim-exists-Prop P Q)

--------------------------------------------------------------------------------

-- Section 14.4 Mapping propositional truncations into sets

--------------------------------------------------------------------------------

-- Example 14.4.1

is-prop-is-lower-bound-ℕ :
  {l1 : Level} {P : ℕ → UU l1} (x : ℕ) → is-prop (is-lower-bound-ℕ P x)
is-prop-is-lower-bound-ℕ x =
  is-prop-Π (λ y → is-prop-function-type (is-prop-leq-ℕ x y))

all-elements-equal-minimal-element-ℕ :
  {l1 : Level} {P : ℕ → UU l1} →
  ((x : ℕ) → is-prop (P x)) → all-elements-equal (minimal-element-ℕ P)
all-elements-equal-minimal-element-ℕ {l1} {P} H (pair x (pair p l)) (pair y (pair q k)) =
  eq-subtype
    ( λ n → is-prop-prod (H n) (is-prop-is-lower-bound-ℕ n))
    ( antisymmetric-leq-ℕ x y (l y q) (k x p))

is-prop-minimal-element-ℕ :
  {l1 : Level} {P : ℕ → UU l1} →
  ((x : ℕ) → is-prop (P x)) → is-prop (minimal-element-ℕ P)
is-prop-minimal-element-ℕ H =
  is-prop-all-elements-equal (all-elements-equal-minimal-element-ℕ H)

minimal-element-ℕ-Prop :
  {l1 : Level} {P : ℕ → UU l1} → ((x : ℕ) → is-prop (P x)) → UU-Prop l1
minimal-element-ℕ-Prop {l1} {P} H =
  pair (minimal-element-ℕ P) (is-prop-minimal-element-ℕ H)

global-choice : {l : Level} → UU l → UU l
global-choice X = type-trunc-Prop X → X

global-choice-equiv :
  {l1 l2 : Level} {X : UU l1} {Y : UU l2} (e : X ≃ Y) →
  global-choice X → global-choice Y
global-choice-equiv e f =
  (map-equiv e ∘ f) ∘ (functor-trunc-Prop (map-inv-equiv e))

global-choice-equiv' :
  {l1 l2 : Level} {X : UU l1} {Y : UU l2} (e : X ≃ Y) →
  global-choice Y → global-choice X
global-choice-equiv' e f =
  (map-inv-equiv e ∘ f) ∘ (functor-trunc-Prop (map-equiv e))

global-choice-decidable-subtype-ℕ :
  {l1 : Level} {P : ℕ → UU l1} (H : (x : ℕ) → is-prop (P x))
  (d : (x : ℕ) → is-decidable (P x)) → global-choice (Σ ℕ P)
global-choice-decidable-subtype-ℕ {l1} {P} H d t =
  tot ( λ x → pr1)
      ( apply-universal-property-trunc-Prop t
        ( minimal-element-ℕ-Prop H)
        ( well-ordering-principle-ℕ P d))

is-prop-is-lower-bound-Fin :
  {l : Level} {k : ℕ} {P : Fin k → UU l} (x : Fin k) →
  is-prop (is-lower-bound-Fin P x)
is-prop-is-lower-bound-Fin x =
  is-prop-Π (λ y → is-prop-function-type (is-prop-leq-Fin x y))

all-elements-equal-minimal-element-Fin :
  {l : Level} {k : ℕ} (P : Fin k → UU l) →
  ((x : Fin k) → is-prop (P x)) → all-elements-equal (minimal-element-Fin P)
all-elements-equal-minimal-element-Fin P H
  (pair x (pair p l)) (pair y (pair q m)) =
  eq-subtype
    ( λ t → is-prop-prod (H t) (is-prop-is-lower-bound-Fin t))
    ( antisymmetric-leq-Fin (l y q) (m x p))

is-prop-minimal-element-Fin :
  {l : Level} {k : ℕ} (P : Fin k → UU l) →
  ((x : Fin k) → is-prop (P x)) → is-prop (minimal-element-Fin P)
is-prop-minimal-element-Fin P H =
  is-prop-all-elements-equal (all-elements-equal-minimal-element-Fin P H)

minimal-element-Fin-Prop :
  {l : Level} {k : ℕ} (P : Fin k → UU l) → ((x : Fin k) → is-prop (P x)) →
  UU-Prop l
minimal-element-Fin-Prop P H =
  pair (minimal-element-Fin P) (is-prop-minimal-element-Fin P H)

global-choice-decidable-subtype-Fin :
  {l : Level} {k : ℕ} (P : Fin k → UU l) → ((x : Fin k) → is-prop (P x)) →
  ((x : Fin k) → is-decidable (P x)) → global-choice (Σ (Fin k) P)
global-choice-decidable-subtype-Fin {l} {zero-ℕ} P H d t =
  ex-falso (apply-universal-property-trunc-Prop t empty-Prop pr1)
global-choice-decidable-subtype-Fin {l} {succ-ℕ k} P H d t =
  map-Σ P
    ( mod-succ-ℕ k)
    ( λ x → id)
    ( global-choice-total-Q
      ( functor-trunc-Prop
        ( map-Σ Q
          ( nat-Fin)
          ( λ x → tr P (inv (issec-nat-Fin x))))
        ( t)))
  where
  Q : ℕ → UU l
  Q n = P (mod-succ-ℕ k n)
  is-prop-Q : (n : ℕ) → is-prop (Q n)
  is-prop-Q n = H (mod-succ-ℕ k n)
  is-decidable-Q : (n : ℕ) → is-decidable (Q n)
  is-decidable-Q n = d (mod-succ-ℕ k n)
  global-choice-total-Q : global-choice (Σ ℕ Q)
  global-choice-total-Q =
    global-choice-decidable-subtype-ℕ is-prop-Q is-decidable-Q

-- Remark 14.4.2

-- We already defined global-choice above

-- Definition 14.4.3

is-weakly-constant-map :
  {l1 l2 : Level} {A : UU l1} {B : UU l2} → (A → B) → UU (l1 ⊔ l2)
is-weakly-constant-map {A = A} f = (x y : A) → Id (f x) (f y)

is-prop-is-weakly-constant-map-Set :
  {l1 l2 : Level} {A : UU l1} (B : UU-Set l2) (f : A → type-Set B) →
  is-prop (is-weakly-constant-map f)
is-prop-is-weakly-constant-map-Set B f =
  is-prop-Π (λ x → is-prop-Π (λ y → is-set-type-Set B (f x) (f y)))

-- Lemma 14.4.4

is-weakly-constant-map-precomp-unit-trunc-Prop :
  {l1 l2 : Level} {A : UU l1} {B : UU l2} (g : type-trunc-Prop A → B) →
  is-weakly-constant-map (g ∘ unit-trunc-Prop)
is-weakly-constant-map-precomp-unit-trunc-Prop g x y =
  ap ( g)
     ( eq-is-prop (is-prop-type-trunc-Prop))

-- Theorem 14.4.5

precomp-universal-property-set-quotient-trunc-Prop :
  {l1 l2 : Level} {A : UU l1} (B : UU-Set l2) →
  (type-trunc-Prop A → type-Set B) → Σ (A → type-Set B) is-weakly-constant-map
precomp-universal-property-set-quotient-trunc-Prop B g =
  pair
    ( g ∘ unit-trunc-Prop)
    ( is-weakly-constant-map-precomp-unit-trunc-Prop g)

all-elements-equal-image-is-weakly-constant-map :
  {l1 l2 : Level} {A : UU l1} (B : UU-Set l2) (f : A → type-Set B) →
  is-weakly-constant-map f →
  all-elements-equal (Σ (type-Set B) (λ b → type-trunc-Prop (fib f b)))
all-elements-equal-image-is-weakly-constant-map B f H (pair x s) (pair y t) =
  eq-subtype
    ( λ b → is-prop-type-trunc-Prop)
    ( apply-universal-property-trunc-Prop s
      ( Id-Prop B x y)
      ( λ u →
        apply-universal-property-trunc-Prop t
          ( Id-Prop B x y)
          ( λ v → inv (pr2 u) ∙ (H (pr1 u) (pr1 v) ∙ pr2 v))))

is-prop-image-is-weakly-constant-map :
  {l1 l2 : Level} {A : UU l1} (B : UU-Set l2) (f : A → type-Set B) →
  is-weakly-constant-map f →
  is-prop (Σ (type-Set B) (λ b → type-trunc-Prop (fib f b)))
is-prop-image-is-weakly-constant-map B f H =
  is-prop-all-elements-equal
    ( all-elements-equal-image-is-weakly-constant-map B f H)

image-weakly-constant-map-Prop :
  {l1 l2 : Level} {A : UU l1} (B : UU-Set l2) (f : A → type-Set B) →
  is-weakly-constant-map f → UU-Prop (l1 ⊔ l2)
image-weakly-constant-map-Prop B f H =
  pair
    ( Σ (type-Set B) (λ b → type-trunc-Prop (fib f b)))
    ( is-prop-image-is-weakly-constant-map B f H)

map-universal-property-set-quotient-trunc-Prop :
  {l1 l2 : Level} {A : UU l1} (B : UU-Set l2) (f : A → type-Set B) →
  is-weakly-constant-map f → type-trunc-Prop A → type-Set B
map-universal-property-set-quotient-trunc-Prop B f H =
  ( pr1) ∘
  ( map-universal-property-trunc-Prop
    ( image-weakly-constant-map-Prop B f H)
    ( λ a → pair (f a) (unit-trunc-Prop (pair a refl))))

map-universal-property-set-quotient-trunc-Prop' :
  {l1 l2 : Level} {A : UU l1} (B : UU-Set l2) →
  Σ (A → type-Set B) is-weakly-constant-map → type-trunc-Prop A → type-Set B
map-universal-property-set-quotient-trunc-Prop' B (pair f H) =
  map-universal-property-set-quotient-trunc-Prop B f H

htpy-universal-property-set-quotient-trunc-Prop :
  {l1 l2 : Level} {A : UU l1} (B : UU-Set l2) (f : A → type-Set B) →
  (H : is-weakly-constant-map f) →
  ( map-universal-property-set-quotient-trunc-Prop B f H ∘ unit-trunc-Prop) ~ f
htpy-universal-property-set-quotient-trunc-Prop B f H a =
  ap ( pr1)
     ( eq-is-prop'
       ( is-prop-image-is-weakly-constant-map B f H)
       ( map-universal-property-trunc-Prop
         ( image-weakly-constant-map-Prop B f H)
         ( λ x → pair (f x) (unit-trunc-Prop (pair x refl)))
         ( unit-trunc-Prop a))
       ( pair (f a) (unit-trunc-Prop (pair a refl))))

issec-map-universal-property-set-quotient-trunc-Prop :
  {l1 l2 : Level} {A : UU l1} (B : UU-Set l2) →
  ( ( precomp-universal-property-set-quotient-trunc-Prop {A = A} B) ∘
    ( map-universal-property-set-quotient-trunc-Prop' B)) ~ id
issec-map-universal-property-set-quotient-trunc-Prop B (pair f H) =
  eq-subtype
    ( is-prop-is-weakly-constant-map-Set B)
    ( eq-htpy (htpy-universal-property-set-quotient-trunc-Prop B f H))

isretr-map-universal-property-set-quotient-trunc-Prop :
  {l1 l2 : Level} {A : UU l1} (B : UU-Set l2) →
  ( ( map-universal-property-set-quotient-trunc-Prop' B) ∘
    ( precomp-universal-property-set-quotient-trunc-Prop {A = A} B)) ~ id
isretr-map-universal-property-set-quotient-trunc-Prop B g =
  eq-htpy
    ( ind-trunc-Prop
      ( λ x →
        Id-Prop B
          ( map-universal-property-set-quotient-trunc-Prop' B
            ( precomp-universal-property-set-quotient-trunc-Prop B g)
            ( x))
          ( g x))
      ( λ x →
        htpy-universal-property-set-quotient-trunc-Prop B
          ( g ∘ unit-trunc-Prop)
          ( is-weakly-constant-map-precomp-unit-trunc-Prop g)
          ( x)))

universal-property-set-quotient-trunc-Prop :
  {l1 l2 : Level} {A : UU l1} (B : UU-Set l2) →
  is-equiv (precomp-universal-property-set-quotient-trunc-Prop {A = A} B)
universal-property-set-quotient-trunc-Prop {A = A} B =
  is-equiv-has-inverse
    ( map-universal-property-set-quotient-trunc-Prop' B)
    ( issec-map-universal-property-set-quotient-trunc-Prop B)
    ( isretr-map-universal-property-set-quotient-trunc-Prop B)

--------------------------------------------------------------------------------

-- Exercises

--------------------------------------------------------------------------------

-- Exercise 14.1

-- Exercise 14.1 (a)

map-trunc-trunc-Prop :
  {l : Level} (A : UU l) →
  type-trunc-Prop (type-trunc-Prop A) → type-trunc-Prop A
map-trunc-trunc-Prop A = map-universal-property-trunc-Prop (trunc-Prop A) id

is-equiv-map-trunc-trunc-Prop :
  {l : Level} (A : UU l) → is-equiv (map-trunc-trunc-Prop A)
is-equiv-map-trunc-trunc-Prop A =
  is-equiv-is-prop
    ( is-prop-type-trunc-Prop)
    ( is-prop-type-trunc-Prop)
    ( unit-trunc-Prop)

is-equiv-unit-trunc-trunc-Prop :
  {l : Level} (A : UU l) → is-equiv (unit-trunc-Prop {A = type-trunc-Prop A})
is-equiv-unit-trunc-trunc-Prop A =
  is-equiv-is-prop
    ( is-prop-type-trunc-Prop)
    ( is-prop-type-trunc-Prop)
    ( map-trunc-trunc-Prop A)

-- Exercise 14.1 (b)

is-inhabited-or-empty : {l1 : Level} → UU l1 → UU l1
is-inhabited-or-empty A = coprod (type-trunc-Prop A) (is-empty A)

is-prop-is-inhabited-or-empty :
  {l1 : Level} (A : UU l1) → is-prop (is-inhabited-or-empty A)
is-prop-is-inhabited-or-empty A =
  is-prop-coprod
    ( λ t → apply-universal-property-trunc-Prop t empty-Prop)
    ( is-prop-type-trunc-Prop)
    ( is-prop-neg)

is-inhabited-or-empty-Prop : {l1 : Level} → UU l1 → UU-Prop l1
is-inhabited-or-empty-Prop A =
  pair (is-inhabited-or-empty A) (is-prop-is-inhabited-or-empty A)

is-prop-is-decidable :
  {l : Level} {A : UU l} → is-prop A → is-prop (is-decidable A)
is-prop-is-decidable is-prop-A =
  is-prop-coprod intro-dn is-prop-A is-prop-neg

is-decidable-Prop :
  {l : Level} → UU-Prop l → UU-Prop l
is-decidable-Prop P =
  pair (is-decidable (type-Prop P)) (is-prop-is-decidable (is-prop-type-Prop P))

is-merely-decidable-Prop :
  {l : Level} → UU l → UU-Prop l
is-merely-decidable-Prop A = trunc-Prop (is-decidable A)

is-merely-decidable : {l : Level} → UU l → UU l
is-merely-decidable A = type-trunc-Prop (is-decidable A)

is-prop-is-decidable-type-trunc-Prop :
  {l : Level} (A : UU l) → is-prop (is-decidable (type-trunc-Prop A))
is-prop-is-decidable-type-trunc-Prop A =
  is-prop-is-decidable is-prop-type-trunc-Prop

is-decidable-type-trunc-Prop : {l : Level} → UU l → UU-Prop l
is-decidable-type-trunc-Prop A =
  pair ( is-decidable (type-trunc-Prop A))
       ( is-prop-is-decidable-type-trunc-Prop A)

is-decidable-type-trunc-Prop-is-merely-decidable :
  {l : Level} (A : UU l) →
  is-merely-decidable A → is-decidable (type-trunc-Prop A)
is-decidable-type-trunc-Prop-is-merely-decidable A =
  map-universal-property-trunc-Prop
    ( is-decidable-type-trunc-Prop A)
    ( f)
  where
  f : is-decidable A → type-Prop (is-decidable-type-trunc-Prop A)
  f (inl a) = inl (unit-trunc-Prop a)
  f (inr f) = inr (map-universal-property-trunc-Prop empty-Prop f)

is-merely-decidable-is-decidable-type-trunc-Prop :
  {l : Level} (A : UU l) →
  is-decidable (type-trunc-Prop A) → is-merely-decidable A
is-merely-decidable-is-decidable-type-trunc-Prop A (inl x) =
   apply-universal-property-trunc-Prop x
     ( is-merely-decidable-Prop A)
     ( unit-trunc-Prop ∘ inl)
is-merely-decidable-is-decidable-type-trunc-Prop A (inr f) =
  unit-trunc-Prop (inr (f ∘ unit-trunc-Prop))

-- Exercise 14.1 (c)

elim-trunc-Prop-is-decidable :
  {l : Level} {A : UU l} → is-decidable A → type-trunc-Prop A → A
elim-trunc-Prop-is-decidable (inl a) x = a
elim-trunc-Prop-is-decidable (inr f) x =
  ex-falso (apply-universal-property-trunc-Prop x empty-Prop f)

-- Exercise 14.1 (d) 

dn-dn-type-trunc-Prop :
  {l : Level} (A : UU l) → ¬¬ (type-trunc-Prop A) → ¬¬ A
dn-dn-type-trunc-Prop A =
  dn-extend (map-universal-property-trunc-Prop (dn-Prop' A) intro-dn)

dn-type-trunc-Prop-dn :
  {l : Level} {A : UU l} → ¬¬ A → ¬¬ (type-trunc-Prop A)
dn-type-trunc-Prop-dn = functor-dn unit-trunc-Prop

-- Exercise 14.2

is-nonempty-is-inhabited :
  {l : Level} {X : UU l} → type-trunc-Prop X → ¬¬ X
is-nonempty-is-inhabited {l} {X} =
  map-universal-property-trunc-Prop (dn-Prop' X) intro-dn

is-fixed-point-is-decidable-is-inhabited :
  {l : Level} {X : UU l} → type-trunc-Prop X → is-decidable X ≃ X
is-fixed-point-is-decidable-is-inhabited {l} {X} t =
  right-unit-law-coprod-is-empty X (¬ X) (is-nonempty-is-inhabited t)

-- Exercise 14.3

merely-Id-Prop :
  {l : Level} {A : UU l} → A → A → UU-Prop l
merely-Id-Prop x y = trunc-Prop (Id x y)

merely-Id : {l : Level} {A : UU l} → A → A → UU l
merely-Id x y = type-trunc-Prop (Id x y)

refl-merely-Id :
  {l : Level} {A : UU l} (x : A) → merely-Id x x
refl-merely-Id x = unit-trunc-Prop refl

symmetric-merely-Id :
  {l : Level} {A : UU l} {x y : A} → merely-Id x y → merely-Id y x
symmetric-merely-Id {x = x} {y} =
  functor-trunc-Prop inv

transitive-merely-Id :
  {l : Level} {A : UU l} {x y z : A} →
  merely-Id y z → merely-Id x y → merely-Id x z
transitive-merely-Id {x = x} {y} {z} p =
  apply-universal-property-trunc-Prop p
    ( hom-Prop (merely-Id-Prop x y) (merely-Id-Prop x z))
    ( λ q → functor-trunc-Prop (λ p → p ∙ q))

-- Exercise 14.4

is-propositional-truncation-prod :
  {l1 l2 l3 l4 : Level}
  {A : UU l1} (P : UU-Prop l2) (f : A → type-Prop P)
  {A' : UU l3} (P' : UU-Prop l4) (f' : A' → type-Prop P') →
  ({l : Level} → is-propositional-truncation l P f) →
  ({l : Level} → is-propositional-truncation l P' f') →
  {l : Level} → is-propositional-truncation l (prod-Prop P P') (map-prod f f')
is-propositional-truncation-prod P f P' f' is-ptr-f is-ptr-f' Q =
  is-equiv-top-is-equiv-bottom-square
    ( ev-pair)
    ( ev-pair)
    ( precomp (map-prod f f') (type-Prop Q))
    ( λ h a a' → h (f a) (f' a'))
    ( refl-htpy)
    ( is-equiv-ev-pair)
    ( is-equiv-ev-pair)
    ( is-equiv-comp'
      ( λ h a a' → h a (f' a'))
      ( λ h a p' → h (f a) p')
      ( is-ptr-f (pair (type-hom-Prop P' Q) (is-prop-type-hom-Prop P' Q)))
      ( is-equiv-map-Π
        ( λ a g a' → g (f' a'))
        ( λ a → is-ptr-f' Q)))

equiv-prod-trunc-Prop :
  {l1 l2 : Level} (A : UU l1) (A' : UU l2) →
  type-equiv-Prop
    ( trunc-Prop (A × A'))
    ( prod-Prop (trunc-Prop A) (trunc-Prop A'))
equiv-prod-trunc-Prop A A' =
  pr1
    ( center
      ( is-uniquely-unique-propositional-truncation
        ( trunc-Prop (A × A'))
        ( prod-Prop (trunc-Prop A) (trunc-Prop A'))
        ( unit-trunc-Prop)
        ( map-prod unit-trunc-Prop unit-trunc-Prop)
        ( is-propositional-truncation-trunc-Prop (A × A'))
        ( is-propositional-truncation-prod
          ( trunc-Prop A)
          ( unit-trunc-Prop)
          ( trunc-Prop A')
          ( unit-trunc-Prop)
          ( is-propositional-truncation-trunc-Prop A)
          ( is-propositional-truncation-trunc-Prop A'))))

map-distributive-trunc-prod-Prop :
  {l1 l2 : Level} {A : UU l1} {B : UU l2} →
  type-trunc-Prop (A × B) → type-trunc-Prop A × type-trunc-Prop B
map-distributive-trunc-prod-Prop {l1} {l2} {A} {B} =
  map-universal-property-trunc-Prop
    ( pair
      ( type-trunc-Prop A × type-trunc-Prop B)
      ( is-prop-prod is-prop-type-trunc-Prop is-prop-type-trunc-Prop))
    ( map-prod unit-trunc-Prop unit-trunc-Prop)

map-inv-distributive-trunc-prod-Prop :
  {l1 l2 : Level} {A : UU l1} {B : UU l2} →
  type-trunc-Prop A × type-trunc-Prop B → type-trunc-Prop (A × B)
map-inv-distributive-trunc-prod-Prop {l1} {l2} {A} {B} t =
  map-universal-property-trunc-Prop
    ( trunc-Prop (A × B))
    ( λ x →
      map-universal-property-trunc-Prop
        ( trunc-Prop (A × B))
        ( unit-trunc-Prop ∘ (pair x))
        ( pr2 t))
    ( pr1 t)

is-equiv-map-distributive-trunc-prod-Prop :
  {l1 l2 : Level} {A : UU l1} {B : UU l2} →
  is-equiv (map-distributive-trunc-prod-Prop {A = A} {B = B})
is-equiv-map-distributive-trunc-prod-Prop {l1} {l2} {A} {B} =
  is-equiv-is-prop
    ( is-prop-type-trunc-Prop)
    ( is-prop-prod is-prop-type-trunc-Prop is-prop-type-trunc-Prop)
    ( map-inv-distributive-trunc-prod-Prop)

distributive-trunc-prod-Prop :
  {l1 l2 : Level} {A : UU l1} {B : UU l2} →
  type-trunc-Prop (A × B) ≃ (type-trunc-Prop A × type-trunc-Prop B)
distributive-trunc-prod-Prop =
  pair map-distributive-trunc-prod-Prop
       is-equiv-map-distributive-trunc-prod-Prop

is-equiv-map-inv-distributive-trunc-prod-Prop :
  {l1 l2 : Level} {A : UU l1} {B : UU l2} →
  is-equiv (map-inv-distributive-trunc-prod-Prop {A = A} {B = B})
is-equiv-map-inv-distributive-trunc-prod-Prop {l1} {l2} {A} {B} =
  is-equiv-is-prop
    ( is-prop-prod is-prop-type-trunc-Prop is-prop-type-trunc-Prop)
    ( is-prop-type-trunc-Prop)
    ( map-distributive-trunc-prod-Prop)

inv-distributive-trunc-prod-Prop :
  {l1 l2 : Level} {A : UU l1} {B : UU l2} →
  ( type-trunc-Prop A × type-trunc-Prop B) ≃ type-trunc-Prop (A × B)
inv-distributive-trunc-prod-Prop =
  pair map-inv-distributive-trunc-prod-Prop
       is-equiv-map-inv-distributive-trunc-prod-Prop

-- Exercise 14.5

-- Exercise 14.5 (a)

is-propositional-truncation-has-section :
  {l l1 l2 : Level} {A : UU l1} (P : UU-Prop l2) (f : A → type-Prop P) →
  (g : type-Prop P → A) → is-propositional-truncation l P f
is-propositional-truncation-has-section {A = A} P f g Q =
  is-equiv-is-prop
    ( is-prop-function-type (is-prop-type-Prop Q))
    ( is-prop-function-type (is-prop-type-Prop Q))
    ( λ h → h ∘ g)

is-propositional-truncation-terminal-map :
  { l l1 : Level} (A : UU l1) (a : A) →
  is-propositional-truncation l unit-Prop (terminal-map {A = A})
is-propositional-truncation-terminal-map A a =
  is-propositional-truncation-has-section
    ( unit-Prop)
    ( terminal-map)
    ( ind-unit a)

-- Exercise 14.5 (b)

is-propositional-truncation-is-equiv :
  {l l1 l2 : Level} (P : UU-Prop l1) (Q : UU-Prop l2) {f : type-hom-Prop P Q} →
  is-equiv f → is-propositional-truncation l Q f
is-propositional-truncation-is-equiv P Q {f} is-equiv-f R =
  is-equiv-precomp-is-equiv f is-equiv-f (type-Prop R)

is-propositional-truncation-map-equiv :
  { l1 l2 : Level} (P : UU-Prop l1) (Q : UU-Prop l2) (e : type-equiv-Prop P Q) →
  ( l : Level) → is-propositional-truncation l Q (map-equiv e)
is-propositional-truncation-map-equiv P Q e l R =
  is-equiv-precomp-is-equiv (map-equiv e) (is-equiv-map-equiv e) (type-Prop R)

is-equiv-is-propositional-truncation :
  {l1 l2 : Level} (P : UU-Prop l1) (Q : UU-Prop l2) {f : type-hom-Prop P Q} →
  ({l : Level} → is-propositional-truncation l Q f) → is-equiv f
is-equiv-is-propositional-truncation P Q {f} H =
  is-equiv-is-equiv-precomp-Prop P Q f H

is-propositional-truncation-id :
  { l1 : Level} (P : UU-Prop l1) →
  ( l : Level) → is-propositional-truncation l P id
is-propositional-truncation-id P l Q = is-equiv-id

-- Exercise 14.6

-- Definition 14.1.9

dependent-universal-property-propositional-truncation :
  ( l : Level) {l1 l2 : Level} {A : UU l1}
  ( P : UU-Prop l2) (f : A → type-Prop P) → UU (lsuc l ⊔ l1 ⊔ l2)
dependent-universal-property-propositional-truncation l {l1} {l2} {A} P f =
  ( Q : type-Prop P → UU-Prop l) → is-equiv (precomp-Π f (type-Prop ∘ Q))

-- Theorem 14.2.2

abstract
  dependent-universal-property-is-propositional-truncation :
    { l1 l2 : Level} {A : UU l1} (P : UU-Prop l2) (f : A → type-Prop P) →
    ( {l : Level} → is-propositional-truncation l P f) →
    ( {l : Level} → dependent-universal-property-propositional-truncation l P f)
  dependent-universal-property-is-propositional-truncation
    {l1} {l2} {A} P f is-ptr-f Q =
    is-fiberwise-equiv-is-equiv-map-Σ
      ( λ (g : A → type-Prop P) → (x : A) → type-Prop (Q (g x)))
      ( precomp f (type-Prop P))
      ( λ h → precomp-Π f (λ p → type-Prop (Q (h p))))
      ( is-ptr-f P)
      ( is-equiv-top-is-equiv-bottom-square
        ( inv-choice-∞
          { C = λ (x : type-Prop P) (p : type-Prop P) → type-Prop (Q p)})
        ( inv-choice-∞
          { C = λ (x : A) (p : type-Prop P) → type-Prop (Q p)})
        ( map-Σ
          ( λ (g : A → type-Prop P) → (x : A) → type-Prop (Q (g x)))
          ( precomp f (type-Prop P))
          ( λ h → precomp-Π f (λ p → type-Prop (Q (h p)))))
        ( precomp f (Σ (type-Prop P) (λ p → type-Prop (Q p))))
        ( ind-Σ (λ h h' → refl))
        ( is-equiv-inv-choice-∞)
        ( is-equiv-inv-choice-∞)
        ( is-ptr-f (Σ-Prop P Q)))
      ( id {A = type-Prop P})

dependent-universal-property-trunc-Prop :
  {l l1 : Level} {A : UU l1} →
  dependent-universal-property-propositional-truncation l
    ( trunc-Prop A)
    ( unit-trunc-Prop)
dependent-universal-property-trunc-Prop {A = A} =
  dependent-universal-property-is-propositional-truncation
    ( trunc-Prop A)
    ( unit-trunc-Prop)
    ( is-propositional-truncation-trunc-Prop A)

equiv-dependent-universal-property-trunc-Prop :
  {l1 l2 : Level} {A : UU l1} (P : type-trunc-Prop A → UU-Prop l2) →
  (((y : type-trunc-Prop A) → type-Prop (P y)) ≃
  ((x : A) → type-Prop (P (unit-trunc-Prop x))))
equiv-dependent-universal-property-trunc-Prop P =
  pair
    ( precomp-Π unit-trunc-Prop (type-Prop ∘ P))
    ( dependent-universal-property-trunc-Prop P)

abstract
  is-propositional-truncation-dependent-universal-property :
    { l1 l2 : Level} {A : UU l1} (P : UU-Prop l2) (f : A → type-Prop P) →
    ( {l : Level} →
      dependent-universal-property-propositional-truncation l P f) →
    ( {l : Level} → is-propositional-truncation l P f)
  is-propositional-truncation-dependent-universal-property P f dup-f Q =
    dup-f (λ p → Q)

-- Exercise 14.7

-- The impredicative encoding of the propositional truncation --

impredicative-trunc-Prop :
  {l : Level} → UU l → UU-Prop (lsuc l)
impredicative-trunc-Prop {l} A =
  Π-Prop
    ( UU-Prop l)
    ( λ Q → function-Prop (A → type-Prop Q) Q)

type-impredicative-trunc-Prop :
  {l : Level} → UU l → UU (lsuc l)
type-impredicative-trunc-Prop {l} A =
  type-Prop (impredicative-trunc-Prop A)

map-impredicative-trunc-Prop :
  {l : Level} (A : UU l) →
  type-trunc-Prop A → type-impredicative-trunc-Prop A
map-impredicative-trunc-Prop {l} A =
  map-universal-property-trunc-Prop
    ( impredicative-trunc-Prop A)
    ( λ x Q f → f x)

inv-map-impredicative-trunc-Prop :
  {l : Level} (A : UU l) →
  type-impredicative-trunc-Prop A → type-trunc-Prop A
inv-map-impredicative-trunc-Prop A H =
  H (trunc-Prop A) unit-trunc-Prop

equiv-impredicative-trunc-Prop :
  {l : Level} (A : UU l) →
  type-trunc-Prop A ≃ type-impredicative-trunc-Prop A
equiv-impredicative-trunc-Prop A =
  equiv-iff
    ( trunc-Prop A)
    ( impredicative-trunc-Prop A)
    ( map-impredicative-trunc-Prop A)
    ( inv-map-impredicative-trunc-Prop A)

-- The impredicative encoding of conjunction --

impredicative-conj-Prop :
  {l1 l2 : Level} → UU-Prop l1 → UU-Prop l2 → UU-Prop (lsuc (l1 ⊔ l2))
impredicative-conj-Prop {l1} {l2} P1 P2 =
  Π-Prop
    ( UU-Prop (l1 ⊔ l2))
    ( λ Q → function-Prop (type-Prop P1 → (type-Prop P2 → type-Prop Q)) Q)

type-impredicative-conj-Prop :
  {l1 l2 : Level} → UU-Prop l1 → UU-Prop l2 → UU (lsuc (l1 ⊔ l2))
type-impredicative-conj-Prop P1 P2 =
  type-Prop (impredicative-conj-Prop P1 P2)

map-impredicative-conj-Prop :
  {l1 l2 : Level} (P1 : UU-Prop l1) (P2 : UU-Prop l2) →
  type-conj-Prop P1 P2 → type-impredicative-conj-Prop P1 P2
map-impredicative-conj-Prop {l1} {l2} P1 P2 (pair p1 p2) Q f =
  f p1 p2

inv-map-impredicative-conj-Prop :
  {l1 l2 : Level} (P1 : UU-Prop l1) (P2 : UU-Prop l2) →
  type-impredicative-conj-Prop P1 P2 → type-conj-Prop P1 P2
inv-map-impredicative-conj-Prop P1 P2 H =
  H (conj-Prop P1 P2) (λ p1 p2 → pair p1 p2)

equiv-impredicative-conj-Prop :
  {l1 l2 : Level} (P1 : UU-Prop l1) (P2 : UU-Prop l2) →
  type-conj-Prop P1 P2 ≃ type-impredicative-conj-Prop P1 P2
equiv-impredicative-conj-Prop P1 P2 =
  equiv-iff
    ( conj-Prop P1 P2)
    ( impredicative-conj-Prop P1 P2)
    ( map-impredicative-conj-Prop P1 P2)
    ( inv-map-impredicative-conj-Prop P1 P2)

-- The impredicative encoding of disjunction --

impredicative-disj-Prop :
  {l1 l2 : Level} → UU-Prop l1 → UU-Prop l2 → UU-Prop (lsuc (l1 ⊔ l2))
impredicative-disj-Prop {l1} {l2} P1 P2 =
  Π-Prop
    ( UU-Prop (l1 ⊔ l2))
    ( λ Q →
      function-Prop
        ( type-implication-Prop P1 Q)
        ( function-Prop (type-implication-Prop P2 Q) Q))

type-impredicative-disj-Prop :
  {l1 l2 : Level} → UU-Prop l1 → UU-Prop l2 → UU (lsuc (l1 ⊔ l2))
type-impredicative-disj-Prop P1 P2 =
  type-Prop (impredicative-disj-Prop P1 P2)

map-impredicative-disj-Prop :
  {l1 l2 : Level} (P1 : UU-Prop l1) (P2 : UU-Prop l2) →
  type-disj-Prop P1 P2 → type-impredicative-disj-Prop P1 P2
map-impredicative-disj-Prop {l1} {l2} P1 P2 =
  map-universal-property-trunc-Prop
    ( impredicative-disj-Prop P1 P2)
    ( ind-coprod
      ( λ x → type-impredicative-disj-Prop P1 P2)
      ( λ x Q f1 f2 → f1 x)
      ( λ y Q f1 f2 → f2 y))
  
inv-map-impredicative-disj-Prop :
  {l1 l2 : Level} (P1 : UU-Prop l1) (P2 : UU-Prop l2) →
  type-impredicative-disj-Prop P1 P2 → type-disj-Prop P1 P2
inv-map-impredicative-disj-Prop P1 P2 H =
  H (disj-Prop P1 P2) (inl-disj-Prop P1 P2) (inr-disj-Prop P1 P2)

equiv-impredicative-disj-Prop :
  {l1 l2 : Level} (P1 : UU-Prop l1) (P2 : UU-Prop l2) →
  type-disj-Prop P1 P2 ≃ type-impredicative-disj-Prop P1 P2
equiv-impredicative-disj-Prop P1 P2 =
  equiv-iff
    ( disj-Prop P1 P2)
    ( impredicative-disj-Prop P1 P2)
    ( map-impredicative-disj-Prop P1 P2)
    ( inv-map-impredicative-disj-Prop P1 P2)

-- The impredicative encoding of negation --

impredicative-neg-Prop :
  {l : Level} → UU l → UU-Prop (lsuc l)
impredicative-neg-Prop {l} A =
  Π-Prop (UU-Prop l) (λ Q → function-Prop A Q)

type-impredicative-neg-Prop :
  {l : Level} → UU l → UU (lsuc l)
type-impredicative-neg-Prop A =
  type-Prop (impredicative-neg-Prop A)

map-impredicative-neg-Prop :
  {l : Level} (A : UU l) →
  ¬ A → type-impredicative-neg-Prop A
map-impredicative-neg-Prop A f Q a = ex-falso (f a)

inv-map-impredicative-neg-Prop :
  {l : Level} (A : UU l) →
  type-impredicative-neg-Prop A → ¬ A
inv-map-impredicative-neg-Prop A H a = H (neg-Prop' A) a a

equiv-impredicative-neg-Prop :
  {l : Level} (A : UU l) →
  ¬ A ≃ type-impredicative-neg-Prop A
equiv-impredicative-neg-Prop A =
  equiv-iff
    ( neg-Prop' A)
    ( impredicative-neg-Prop A)
    ( map-impredicative-neg-Prop A)
    ( inv-map-impredicative-neg-Prop A)

-- The impredicative encoding of existential quantification --

impredicative-exists-Prop :
  {l1 l2 : Level} {A : UU l1} (P : A → UU-Prop l2) → UU-Prop (lsuc (l1 ⊔ l2))
impredicative-exists-Prop {l1} {l2} {A} P =
  Π-Prop
    ( UU-Prop (l1 ⊔ l2))
    ( λ Q → function-Prop ((x : A) → type-Prop (P x) → type-Prop Q) Q)

type-impredicative-exists-Prop :
  {l1 l2 : Level} {A : UU l1} (P : A → UU-Prop l2) → UU (lsuc (l1 ⊔ l2))
type-impredicative-exists-Prop P =
  type-Prop (impredicative-exists-Prop P)

map-impredicative-exists-Prop :
  {l1 l2 : Level} {A : UU l1} (P : A → UU-Prop l2) →
  exists P → type-impredicative-exists-Prop P
map-impredicative-exists-Prop {l1} {l2} {A} P =
  map-universal-property-trunc-Prop
    ( impredicative-exists-Prop P)
    ( ind-Σ (λ x y Q h → h x y))

inv-map-impredicative-exists-Prop :
  {l1 l2 : Level} {A : UU l1} (P : A → UU-Prop l2) →
  type-impredicative-exists-Prop P → exists P
inv-map-impredicative-exists-Prop {A = A} P H =
  H ( exists-Prop P)
    ( λ x y → unit-trunc-Prop (pair x y))

equiv-impredicative-exists-Prop :
  {l1 l2 : Level} {A : UU l1} (P : A → UU-Prop l2) →
  exists P ≃ type-impredicative-exists-Prop P
equiv-impredicative-exists-Prop P =
  equiv-iff
    ( exists-Prop P)
    ( impredicative-exists-Prop P)
    ( map-impredicative-exists-Prop P)
    ( inv-map-impredicative-exists-Prop P)

-- The impredicative encoding of the based identity type of a set --

impredicative-based-id-Prop :
  {l : Level} (A : UU-Set l) (a x : type-Set A) → UU-Prop (lsuc l)
impredicative-based-id-Prop {l} A a x =
  Π-Prop (type-Set A → UU-Prop l) (λ Q → hom-Prop (Q a) (Q x))

type-impredicative-based-id-Prop :
  {l : Level} (A : UU-Set l) (a x : type-Set A) → UU (lsuc l)
type-impredicative-based-id-Prop A a x =
  type-Prop (impredicative-based-id-Prop A a x)

map-impredicative-based-id-Prop :
  {l : Level} (A : UU-Set l) (a x : type-Set A) →
  Id a x → type-impredicative-based-id-Prop A a x
map-impredicative-based-id-Prop A a .a refl Q p = p

inv-map-impredicative-based-id-Prop :
  {l : Level} (A : UU-Set l) (a x : type-Set A) →
  type-impredicative-based-id-Prop A a x → Id a x
inv-map-impredicative-based-id-Prop A a x H =
  H (λ x → pair (Id a x) (is-set-type-Set A a x)) refl

equiv-impredicative-based-id-Prop :
  {l : Level} (A : UU-Set l) (a x : type-Set A) →
  Id a x ≃ type-impredicative-based-id-Prop A a x
equiv-impredicative-based-id-Prop A a x =
  equiv-iff
    ( pair (Id a x) (is-set-type-Set A a x))
    ( impredicative-based-id-Prop A a x)
    ( map-impredicative-based-id-Prop A a x)
    ( inv-map-impredicative-based-id-Prop A a x)

-- The impredicative encoding of Martin-Löf's identity type of a set --

impredicative-id-Prop :
  {l : Level} (A : UU-Set l) (x y : type-Set A) → UU-Prop (lsuc l)
impredicative-id-Prop {l} A x y =
  Π-Prop (type-Set A → type-Set A → UU-Prop l)
    (λ Q → function-Prop ((a : type-Set A) → type-Prop (Q a a)) (Q x y))

type-impredicative-id-Prop :
  {l : Level} (A : UU-Set l) (x y : type-Set A) → UU (lsuc l)
type-impredicative-id-Prop A x y =
  type-Prop (impredicative-id-Prop A x y)

map-impredicative-id-Prop :
  {l : Level} (A : UU-Set l) (x y : type-Set A) →
  Id x y → type-impredicative-id-Prop A x y
map-impredicative-id-Prop A x .x refl Q r = r x

inv-map-impredicative-id-Prop :
  {l : Level} (A : UU-Set l ) (x y : type-Set A) →
  type-impredicative-id-Prop A x y → Id x y
inv-map-impredicative-id-Prop A x y H =
  H (λ a b → pair (Id a b) (is-set-type-Set A a b)) (λ a → refl)

equiv-impredicative-id-Prop :
  {l : Level} (A : UU-Set l) (x y : type-Set A) →
  Id x y ≃ type-impredicative-id-Prop A x y
equiv-impredicative-id-Prop A x y =
  equiv-iff
    ( pair (Id x y) (is-set-type-Set A x y))
    ( impredicative-id-Prop A x y)
    ( map-impredicative-id-Prop A x y)
    ( inv-map-impredicative-id-Prop A x y)

-- Exercise 14.8

--------------------------------------------------------------------------------

postulate 𝕀 : UU lzero

postulate source-𝕀 : 𝕀

postulate target-𝕀 : 𝕀

postulate path-𝕀 : Id source-𝕀 target-𝕀

postulate ind-𝕀 : {l : Level} (P : 𝕀 → UU l) (u : P source-𝕀) (v : P target-𝕀) (q : Id (tr P path-𝕀 u) v) → (x : 𝕀) → P x

postulate comp-source-𝕀 : {l : Level} {P : 𝕀 → UU l} (u : P source-𝕀) (v : P target-𝕀) (q : Id (tr P path-𝕀 u) v) → Id (ind-𝕀 P u v q source-𝕀) u

postulate comp-target-𝕀 : {l : Level} {P : 𝕀 → UU l} (u : P source-𝕀) (v : P target-𝕀) (q : Id (tr P path-𝕀 u) v) → Id (ind-𝕀 P u v q target-𝕀) v

postulate comp-path-𝕀 : {l : Level} {P : 𝕀 → UU l} (u : P source-𝕀) (v : P target-𝕀) (q : Id (tr P path-𝕀 u) v) → Id (apd (ind-𝕀 P u v q) path-𝕀 ∙ comp-target-𝕀 u v q) (ap (tr P path-𝕀) (comp-source-𝕀 u v q) ∙ q)

Data-𝕀 : {l : Level} → (𝕀 → UU l) → UU l
Data-𝕀 P = Σ (P source-𝕀) (λ u → Σ (P target-𝕀) (λ v → Id (tr P path-𝕀 u) v))

ev-𝕀 : {l : Level} {P : 𝕀 → UU l} → ((x : 𝕀) → P x) → Data-𝕀 P
ev-𝕀 f = triple (f source-𝕀) (f target-𝕀) (apd f path-𝕀)

Eq-Data-𝕀 : {l : Level} {P : 𝕀 → UU l} (x y : Data-𝕀 P) → UU l
Eq-Data-𝕀 {l} {P} x y =
  Σ ( Id (pr1 x) (pr1 y)) (λ α →
     Σ ( Id (pr1 (pr2 x)) (pr1 (pr2 y))) (λ β →
       Id ( pr2 (pr2 x) ∙ β) ( (ap (tr P path-𝕀) α) ∙ pr2 (pr2 y))))

refl-Eq-Data-𝕀 : {l : Level} {P : 𝕀 → UU l} (x : Data-𝕀 P) → Eq-Data-𝕀 x x
refl-Eq-Data-𝕀 x = triple refl refl right-unit

Eq-eq-Data-𝕀 :
  {l : Level} {P : 𝕀 → UU l} {x y : Data-𝕀 P} → Id x y → Eq-Data-𝕀 x y
Eq-eq-Data-𝕀 {x = x} refl = refl-Eq-Data-𝕀 x

is-contr-total-Eq-Data-𝕀 :
  {l : Level} {P : 𝕀 → UU l} (x : Data-𝕀 P) →
  is-contr (Σ (Data-𝕀 P) (Eq-Data-𝕀 x))
is-contr-total-Eq-Data-𝕀 {l} {P} x =
  is-contr-total-Eq-structure
    ( λ u vq α →
      Σ ( Id (pr1 (pr2 x)) (pr1 vq))
        ( λ β → Id (pr2 (pr2 x) ∙ β) (ap (tr P path-𝕀) α ∙ pr2 vq)))
    ( is-contr-total-path (pr1 x))
    ( pair (pr1 x) refl)
    ( is-contr-total-Eq-structure
      ( λ v q β → Id (pr2 (pr2 x) ∙ β) q)
      ( is-contr-total-path (pr1 (pr2 x)))
      ( pair (pr1 (pr2 x)) refl)
      ( is-contr-total-path (pr2 (pr2 x) ∙ refl)))

is-equiv-Eq-eq-Data-𝕀 :
  {l : Level} {P : 𝕀 → UU l} (x y : Data-𝕀 P) →
  is-equiv (Eq-eq-Data-𝕀 {x = x} {y})
is-equiv-Eq-eq-Data-𝕀 x =
  fundamental-theorem-id x
    ( refl-Eq-Data-𝕀 x)
    ( is-contr-total-Eq-Data-𝕀 x)
    ( λ y → Eq-eq-Data-𝕀 {_} {_} {x} {y})

eq-Eq-Data-𝕀' :
  {l : Level} {P : 𝕀 → UU l} {x y : Data-𝕀 P} → Eq-Data-𝕀 x y → Id x y
eq-Eq-Data-𝕀' {l} {P} {x} {y} = map-inv-is-equiv (is-equiv-Eq-eq-Data-𝕀 x y)

eq-Eq-Data-𝕀 :
  {l : Level} {P : 𝕀 → UU l} {x y : Data-𝕀 P} (α : Id (pr1 x) (pr1 y))
  (β : Id (pr1 (pr2 x)) (pr1 (pr2 y)))
  (γ : Id (pr2 (pr2 x) ∙ β) (ap (tr P path-𝕀) α ∙ pr2 (pr2 y))) →
  Id x y
eq-Eq-Data-𝕀 α β γ = eq-Eq-Data-𝕀' (triple α β γ)

inv-ev-𝕀 : {l : Level} {P : 𝕀 → UU l} → Data-𝕀 P → (x : 𝕀) → P x
inv-ev-𝕀 x = ind-𝕀 _ (pr1 x) (pr1 (pr2 x)) (pr2 (pr2 x))

issec-inv-ev-𝕀 : {l : Level} {P : 𝕀 → UU l} (x : Data-𝕀 P) →
  Id (ev-𝕀 (inv-ev-𝕀 x)) x
issec-inv-ev-𝕀 (pair u (pair v q)) =
  eq-Eq-Data-𝕀
    ( comp-source-𝕀 u v q)
    ( comp-target-𝕀 u v q)
    ( comp-path-𝕀 u v q)

tr-value :
  {l1 l2 : Level} {A : UU l1} {B : A → UU l2} (f g : (x : A) → B x) {x y : A}
  (p : Id x y) (q : Id (f x) (g x)) (r : Id (f y) (g y)) →
  Id (apd f p ∙ r) (ap (tr B p) q ∙ apd g p) → Id (tr (λ x → Id (f x) (g x)) p q) r
tr-value f g refl q r s = (inv (ap-id q) ∙ inv right-unit) ∙ inv s

isretr-inv-ev-𝕀 :
  {l : Level} {P : 𝕀 → UU l} (f : (x : 𝕀) → P x) → Id (inv-ev-𝕀 (ev-𝕀 f)) f
isretr-inv-ev-𝕀 {l} {P} f =
  eq-htpy
    ( ind-𝕀
      ( λ x → Id (inv-ev-𝕀 (ev-𝕀 f) x) (f x))
      ( comp-source-𝕀 (f source-𝕀) (f target-𝕀) (apd f path-𝕀))
      ( comp-target-𝕀 (f source-𝕀) (f target-𝕀) (apd f path-𝕀))
      ( tr-value (inv-ev-𝕀 (ev-𝕀 f)) f path-𝕀
        ( comp-source-𝕀 (f source-𝕀) (f target-𝕀) (apd f path-𝕀))
        ( comp-target-𝕀 (f source-𝕀) (f target-𝕀) (apd f path-𝕀))
        ( comp-path-𝕀 (f source-𝕀) (f target-𝕀) (apd f path-𝕀))))

is-equiv-ev-𝕀 :
  {l : Level} (P : 𝕀 → UU l) → is-equiv (ev-𝕀 {P = P})
is-equiv-ev-𝕀 P =
  is-equiv-has-inverse inv-ev-𝕀 issec-inv-ev-𝕀 isretr-inv-ev-𝕀

tr-eq : {l : Level} {A : UU l} {x y : A} (p : Id x y) → Id (tr (Id x) p refl) p
tr-eq refl = refl

contraction-𝕀 : (x : 𝕀) → Id source-𝕀 x
contraction-𝕀 =
  ind-𝕀
    ( Id source-𝕀)
    ( refl)
    ( path-𝕀)
    ( tr-eq path-𝕀)

is-contr-𝕀 : is-contr 𝕀
is-contr-𝕀 = pair source-𝕀 contraction-𝕀

-----------

is-empty-type-trunc-Prop :
  {l1 : Level} {X : UU l1} → is-empty X → is-empty (type-trunc-Prop X)
is-empty-type-trunc-Prop f =
  map-universal-property-trunc-Prop empty-Prop f

is-empty-type-trunc-Prop' :
  {l1 : Level} {X : UU l1} → is-empty (type-trunc-Prop X) → is-empty X
is-empty-type-trunc-Prop' f = f ∘ unit-trunc-Prop

elim-trunc-decidable-fam-Fin :
  {l1 : Level} {k : ℕ} {B : Fin k → UU l1} →
  ((x : Fin k) → is-decidable (B x)) →
  type-trunc-Prop (Σ (Fin k) B) → Σ (Fin k) B
elim-trunc-decidable-fam-Fin {l1} {zero-ℕ} {B} d y =
  ex-falso (is-empty-type-trunc-Prop pr1 y)
elim-trunc-decidable-fam-Fin {l1} {succ-ℕ k} {B} d y
  with d (inr star)
... | inl x = pair (inr star) x
... | inr f =
  map-Σ-map-base inl B
    ( elim-trunc-decidable-fam-Fin {l1} {k} {B ∘ inl}
      ( λ x → d (inl x))
      ( map-equiv-trunc-Prop
        ( ( ( right-unit-law-coprod-is-empty
              ( Σ (Fin k) (B ∘ inl))
              ( B (inr star)) f) ∘e
            ( equiv-coprod equiv-id (left-unit-law-Σ (B ∘ inr)))) ∘e
          ( right-distributive-Σ-coprod (Fin k) unit B))
        ( y)))
